ImpCorrectnessTest updated to test compile_aexp_correct

src/coq/ImpCorrectnessTest.v
@@ -1,8 +1,11 @@
 (* QuickChick dependencies *)
 Require Import QuickChick.QuickChick.
 Import QcDefaultNotation. Open Scope qc_scope.
+Import QcDoNotation.
 
 Require Import ZArith.
+Require Import String.
+Require Import Sumbool.
 
 (* CompCert dependencies *)
 Require Import compcert.lib.Integers.
@@ -26,18 +29,44 @@ Require Import Program.
 (* Verification File *)
 Require Import Vellvm.ImpCorrectness.
 
-
 (* Derive ArbitrarySizedSuchThat for (fun a : aexp => aevalR test_state a n). *)
 
-Fixpoint is_prefix_of {A : Type} `{eq_dec A} (l1 l2 : list A) : bool :=
-  match l1, l2 with
-  | [], _ => true
-  | (x :: xs), (y :: ys) =>
-    if decide (x = y) then
-      is_prefix_of xs ys else
-      false
-  | _, _ => false
-  end.
+Inductive prefix_of {A : Type}: list A -> list A -> Prop :=
+| prefix_nil : forall l : list A, prefix_of [] l
+| prefix_cons_same : forall a l1 l2, prefix_of l1 l2 -> prefix_of (a :: l1) (a :: l2).
+
+Inductive suffix_of {A : Type}: list A -> list A -> Prop :=
+| suffix_nil : forall l : list A, suffix_of l []
+| suffix_app : forall a l1 l2, suffix_of l1 l2 -> suffix_of (l1 ++ [a]) (l2 ++ [a]).
+
+Instance dec_prefix_of : forall A `{eq_dec A} (l1 l2 : list A), Decidable (prefix_of l1 l2).
+Proof.
+  intros A A_decidable.
+  induction l1 as [| a l1']; unfold Decidable.
+  - intros [| a l2']; left; constructor.
+  - intros [| b l2']; try solve [right; intros H; inversion H].
+    refine
+      (match a == b with
+       | left _ =>
+         match decide (prefix_of l1' l2') with
+         | left tail_eq => _
+         | right tail_neq => right _
+         end
+       | right head_neq => right _
+       end).
+    { subst; constructor. constructor. tauto. }
+    { intros H. apply tail_neq. inversion H; subst; auto. }
+    { intros H. apply head_neq. inversion H; subst; auto. }
+Defined.
+
+Instance dec_Z_leq : forall n m : int, Decidable (n <= m)%Z.
+Proof.
+  unfold Decidable. intros n m.
+  destruct (n <=? m)%Z eqn:n_m.
+  - left; rewrite Z.leb_le in n_m; auto.
+  - right; intros H; rewrite <- Z.leb_le in H;
+      rewrite n_m in H; inversion H.
+Defined.
 
 Definition compile_aexp_monotonic_aux
            (g : ctxt) (a : aexp) (n m : int) (code: list elt)
@@ -45,8 +74,12 @@ Definition compile_aexp_monotonic_aux
     let '((n', m', code'), v_opt) := compile_aexp g a (n,m,code) in
     match v_opt with
     | inl err => false
-    | inr v' => andb (andb (Z.leb n n') (Z.leb m m'))
-                    (is_prefix_of (List.rev code) (List.rev code'))
+    | inr v' =>
+      andb (andb (Z.leb n n') (Z.leb m m'))
+           (match decide (prefix_of (List.rev code) (List.rev code')) with
+            | left _ => true
+            | right _ => false
+            end)
     end.
 
 Definition test_compile_aexp_monotonic (a : aexp) (n m : int) :=
@@ -59,70 +92,629 @@ Definition test_compile_aexp_monotonic (a : aexp) (n m : int) :=
     checker (compile_aexp_monotonic_aux new_context a n' m' c)
   end.
 
-
 (*! Section TestCompileAexpMonotonic *)
 
 Existing Instance genSaexp.
 
-(*! QuickChick (forAll arbitrary test_compile_aexp_monotonic). *)
+Definition test_compile_aexp_monotonic_wrapper :=
+  forAll arbitrary test_compile_aexp_monotonic.
+
+(*! QuickChick test_compile_aexp_monotonic_wrapper. *)
 
 Remove Hints genSaexp : typeclass_instances.
 (* End Section *)
 
+Definition bundled_memory := ((list id) * ctxt * env * memory * Imp.state)%type.
+
+Definition satisfies_memory_invariant_and_bound (m : bundled_memory) (n : int) : Prop :=
+  match m with
+  | (_, c, e, mem, s) => memory_invariant c e mem s /\ env_lt n e
+  end.
+
+Fixpoint check_env_lt (n : int) (e : env) : bool :=
+  match e with
+  | [] => true
+  | (Raw local_id, _) :: rest =>
+    if Z.ltb local_id n then check_env_lt n rest
+    else false
+  | _ => false
+  end.
+
+Fixpoint check_memory_invariant (m : bundled_memory) :=
+  match m with
+  | ([], _, _, _, _) => true
+  | (Id var :: vars, c, e, mem, st) =>
+    match lookup_env e (Name var) with
+    | Some (DVALUE_Addr a) =>
+      if (List.nth_default undef mem a) == DVALUE_I64 (st (Id var)) then true
+      else false
+    | _ => false
+    end
+  end.
+
+Definition check_memory_invariant_and_bound (m : bundled_memory) (n : int) : bool :=
+  match m with
+  | (vars, c, e, mem, s) =>
+    andb (check_memory_invariant (vars, c, e, mem, s))
+         (check_env_lt n e)
+  end.
+
+Definition aexp_correct_relation1
+           (vars : list id) (g : ctxt) (e: env) (st : Imp.state) 
+           (bound : int) (v : Ollvm_ast.value) (ans : int64)
+           (k : stack) (fn : function_id) (bid: block_id)
+           (phis : list (local_id * phi)) (term : (instr_id * terminator))
+           (s : SS.state) (mem : memory) :=
+  let '(pc', e', k') := s in
+  pc' = slc_pc fn bid phis term [] /\
+  satisfies_memory_invariant_and_bound (vars, g, e', mem, st) bound /\
+  Rv64e (eval_op e' (Some (TYPE_I 64)%Z) v) ans /\
+  env_extends e e'.
+
+Definition aexp_correct_relation2
+           (vars : list id) (g : ctxt) (e: env) (st : Imp.state) 
+           (bound : int) (v : Ollvm_ast.value) (ans : int64)
+           (k : stack) (fn : function_id) (bid : block_id)
+           (phis : list (local_id * phi)) (term : (instr_id * terminator))
+           (s : SS.state) (mem : memory) :=
+  let '(pc', e', k') := s in  
+  satisfies_memory_invariant_and_bound (vars, g, e', mem, st) bound.
+
+Definition get_compiled_prefix `{eq_dec A} (code_before code_after : list A) :=
+  let fix get_suffix l1 l2 :=
+      match l1, l2 with
+      | (x :: xs), (y :: ys) =>
+        if x == y then
+          get_suffix xs ys
+        else None
+      | [], ys => Some ys
+      | _, _ => None
+      end
+  in match (get_suffix (List.rev code_before) (List.rev code_after)) with
+     | Some l => Some (List.rev l)
+     | None => None
+     end.
+
+Fixpoint compiled_code_of (elts : list elt) :=
+  match elts with
+  | [] => Some []
+  | I id instr :: tl =>
+    match compiled_code_of tl with
+    | Some tl' => Some ((id, instr) :: tl')
+    | None => None
+    end
+  | _ => None
+  end.
+
+Definition empty_cfg : cfg :=
+  {| init := Name "start" ; blks := (fun blk => None); glbl := [] |}.
+
+
+(***************** Goals: *************************************************************
+Lemma compile_aexp_correct :
+  forall 
+    (a:aexp) (st:Imp.state) (ans:int64)
+    (HAexp: aeval st a = ans)
+
+    (g:ctxt)
+    (n m:int) (cd:list elt)
+    (n' m':int) (cd':list elt)
+    (v : Ollvm_ast.value)
+    (Hcomp : compile_aexp g a (n,m,cd) = ((n',m',cd'),inr v)),
+
+  exists cd_a c_a,
+    cd' = cd_a ++ cd
+    /\ compiled_code cd_a c_a
+    /\ straight c_a
+    /\ forall
+    (e:env)
+    (mem:memory) (Hlt:env_lt n e)
+    (HM: memory_invariant g e mem st)
+    (k:stack)
+    (CFG : mcfg) (fn : function_id) (bid: block_id) phis term,
+      step_code
+        CFG
+        (fun s' mem' =>
+           let '(pc', e', k') := s' in
+           pc' = slc_pc fn bid phis term [] /\
+           memory_invariant g e' mem' st /\
+           Rv64e (eval_op e' (Some (TYPE_I 64)) v) ans /\
+           env_extends e e' /\
+           env_lt n' e'
+        )
+        (List.rev c_a)
+        (slc_pc fn bid phis term (List.rev c_a), e, k) mem.
+
+Notes: 
+- Prenexification
+- Functional dependence of exists
+- Further constraints after exists
+- Dependent generation (e.g. CFG that satisfies a property most of the time, 
+  but not all the time)
+- Adopting the discipline of having Decidable propositions everywhere,
+  so that both generation and testing use one copy. 
+- Higher-order constructs are difficult, e.g. continuation for effects and
+  partial maps for Imp.state. 
+
+Lemma compile_aexp_correct_simple1:
+  forall (a : aexp) (st : Imp.state) (g : ctxt)
+    (e : env) (mem : memory) (vars : list id)
+    (n m : int) (cd : list elt)
+    (n' m' : int) (cd' : list elt) (v_err : err Ollvm_ast.value),
+    (* Simplification: restriction to compatible e, m *) 
+    satisfies_memory_invariant_and_bound (vars, g, e, mem, st) n /\
+    compile_aexp g a (n, m, cd) = ((n', m', cd'), v_err) ->
+    match v_err with
+    | inl err => True (* Says nothing *)
+    | inr v =>       
+      let cd_a := get_compiled_prefix cd cd' in
+      match cd_a with
+      | None => False
+      | Some cd_a =>
+        let c_a := compiled_code_of cd_a in
+        match c_a with
+        | None => False
+        | Some c_a => 
+          (forall (k : stack) (CFG: mcfg) (fn : function_id) (bid: block_id) phis term,
+              step_code CFG
+                        (aexp_correct_relation1 vars g e st n' v
+                                                (aeval st a)
+                                                k fn bid phis term)
+                        (List.rev c_a)
+                        (slc_pc fn bid phis term c_a, e, k)
+                        mem)
+        end
+      end
+    end.
+
+Lemma compile_aexp_correct_simple2:
+  forall (a : aexp) (st : Imp.state) (g : ctxt)
+    (e : env) (mem : memory) (vars : list id)
+    (n m : int) (cd : list elt)
+    (n' m' : int) (cd' : list elt) (v_err : err Ollvm_ast.value),
+    satisfies_memory_invariant_and_bound (vars, g, e, mem, st) n /\
+    compile_aexp g a (n, m, cd) = ((n', m', cd'), v_err) ->
+    match v_err with
+    | inl err => True (* Says nothing *)
+    | inr v =>       
+      let cd_a := get_compiled_prefix cd cd' in
+      match cd_a with
+      | None => False
+      | Some cd_a =>
+        let c_a := compiled_code_of cd_a in
+        match c_a with
+        | None => False
+        | Some c_a => 
+          (forall (k : stack) (CFG: mcfg) (fn : function_id) (bid: block_id) phis term,
+              step_code CFG
+                        (aexp_correct_relation2 vars g e st n' v
+                                                (aeval st a)
+                                                k fn bid phis term)
+                        (List.rev c_a)
+                        (slc_pc fn bid phis term c_a, e, k)
+                        mem)
+        end
+      end
+    end.
+
+Lemma compile_aexp_correct_simple2A:
+  forall (a : aexp) (st : Imp.state) (g : ctxt)
+    (e : env) (mem : memory) (vars : list id)
+    (v_err : err Ollvm_ast.value),
+    satisfies_memory_invariant_and_bound (vars, g, e, mem, st) n /\
+    compile_aexp g a (0, 0, cd) = ((n', m', cd'), v_err) ->
+    match v_err with
+    | inl err => True (* Says nothing *)
+    | inr v =>       
+      let cd_a := get_compiled_prefix [] cd' in
+      match cd_a with
+      | None => False
+      | Some cd_a =>
+        let c_a := compiled_code_of cd_a in
+        match c_a with
+        | None => False
+        | Some c_a => 
+          (forall (k : stack) (fn : function_id) (bid: block_id) phis term,
+              step_code (fixed cfg...)
+                        (aexp_correct_relation2 vars g e st n' v
+                                                (aeval st a)
+                                                k fn bid phis term)
+                        (List.rev c_a)
+                        (slc_pc fn bid phis term c_a, e, k)
+                        mem)
+        end
+      end
+    end.
+****)
+
+Definition aexp_correct_relation_bool2
+           (vars : list id) (g : ctxt) (e: env) (st : Imp.state) 
+           (bound : int) (v : Ollvm_ast.value) (ans : int64)
+           (k : stack) (fn : function_id) (bid : block_id)
+           (phis : list (local_id * phi)) (term : (instr_id * terminator))
+           (s : SS.state) (mem : memory) : bool :=
+  let '(pc', e', k') := s in  
+  check_memory_invariant_and_bound (vars, g, e', mem, st) bound.
+
+Definition inject_into_tle elts :=
+  'blocks <- blocks_of_elts (Anon 0)%Z elts;
+    mret
+   ([
+    TLE_Definition
+    {|
+    df_prototype := imp_decl;
+    df_args := [];
+    df_instrs := blocks
+    |}]).
+
+Definition build_mcfg elts :=
+  match inject_into_tle elts with
+  | inl err => None
+  | inr entities => 
+    let m := modul_of_toplevel_entities entities in
+    mcfg_of_modul m
+  end.
+
+Instance dec_is_Op : forall (i : instr), Decidable (is_Op i).
+Proof.
+  intros i; unfold Decidable; destruct i;
+    try solve [right; intros H; inversion H; auto];
+    try solve [left; constructor].
+Defined.
+
+Instance dec_is_Eff : forall (i : instr), Decidable (is_Eff i).
+Proof.
+  intros i; unfold Decidable; destruct i;
+    try solve [right; intros H; inversion H; auto];
+    try solve [left; constructor].
+Defined.
 
 (*
-Open Scope nat.
-Inductive is_even : nat -> Prop :=
-| even_O: is_even O
-| even_S: forall n : nat, is_even n -> is_even (S (S n)).
-Derive ArbitrarySizedSuchThat for (fun n => is_even n).
+Instance dec_stepD_is_Step : forall CFG (s s' : SS.state), Decidable (stepD CFG s = Step s').
+Proof.
+  intros CFG [[p e] stk] s'.
+  set (fetched := fetch p).
+  destruct p as [fn_id [bid phis code [iid term]]]; unfold Decidable;
+    try solve [intros H; inversion H].
+  unfold fetch in fetched; simpl in fetched.
+  destruct code; simpl; unfold stepD.
+  { destruct term;
+      try solve [right; simpl; intros H; inversion H].
+    { right;
+        simpl;
+        destruct stk;
+        destruct v;
+        unfold lift_err_d;
+        destruct (eval_op e (Some t) v);
+        intros H; try solve [inversion H].
+      destruct f; inversion H.
+    }
+    { right;
+        simpl;
+        destruct stk;
+        intros H; try solve [inversion H].
+      destruct f; inversion H.
+    }
+    { right;
+        simpl;
+        destruct v;
+        unfold lift_err_d.
+      destruct (eval_op e (Some t) v) as [ | b].
+      { intros H; inversion H. }
+      { destruct b;
+          try solve [intros H; inversion H].
+        destruct (Int1.eq x Int1.one); destruct trywith;
+          try solve [intros H; inversion H].
+        destruct trywith;
+          try solve [intros H; inversion H].
+        destruct jump;
+          solve [intros H; inversion H].
+        destruct trywith;
+          try solve [intros H; inversion H];
+          try solve [destruct jump; intros H; inversion H].
+      }       
+    }
+    { right;
+        simpl;
+        unfold lift_err_d;
+        destruct trywith;
+        try solve [intros H; inversion H].
+      destruct trywith;
+        try solve [intros H; inversion H].
+      destruct jump;
+        try solve [intros H; inversion H].
+    }
+  }
+  { destruct p as [i insn].
+    destruct i as [[s | i | i] | i].
+    { destruct insn;
+        unfold lift_err_d;
+        try solve [right; intros H; inversion H].
+      { destruct eval_op;
+          try solve [right; intros H; inversion H].
+        left; destruct s' as [[p' e'] stk'].
+        unfold add_env.
+        
 
-Remove Hints gen_small_typ : typeclass_instances.
-
-
-Derive ArbitrarySizedSuchThat for (fun instr => is_Op instr).
-Print GenSizedSuchThatis_Op.
-Sample (genST (fun i => is_Op i)).
-Sample (@arbitraryST 
-
-Instance gen_instr_op : GenSizedSuchThat instr (fun instr => is_Op instr) :=
-  {| arbitrarySizeST n :=
-       (liftGen Some (liftGen INSTR_Op (arbitrarySized n)))
-  |}.
-
-Sample (genST (fun i => is_Op i)).
+        repeat destruct s'.
+        simpl.
+      
+    Print instr_id.
+    Print raw_id.
+    
+    destruct i.
+    { destruct i0.
 *)
 
+Fixpoint step_code_bool (CFG : mcfg) (R : SS.state -> memory -> bool)
+         (cs : code) (st : SS.state) (mem : memory) : bool :=
+  match cs, st, mem with
+  | [], s, m => if R s m then true else false
+  | (id, i) :: cd, s, m =>
+    if decide (is_Op i) then
+      (* missing prefix test *)
+      match stepD CFG s with
+      | Step s' => step_code_bool CFG R cd s' m
+      | _ => false
+      end
+    else
+      if decide (is_Eff i) then
+        (* missing prefix test *)
+        match stepD CFG s with
+        | Obs (Eff e) =>
+          match mem_step e m with
+          | inr (m', v, k) =>
+            step_code_bool CFG R cd (k v) m'
+          | inl _ => false
+          end
+        | _ => false
+        end
+      else true
+  end.
 
+Existing Instance gen_adhoc_aexp.
+
+Instance show_bundled_memory : Show bundled_memory :=
+  {| show x := 
+       match x with
+       | (ids, c, e, m, s) =>
+         ("vars: " ++ (show ids) ++ "; " ++
+                   "env: " ++ (show e) ++ "; " ++
+                   "mem: " ++ (show m) ++ "; ")%string
+       end
+  |}.
+
+Instance gen_consistent_memory (bound : int):
+  GenSizedSuchThat bundled_memory (fun m => satisfies_memory_invariant_and_bound m bound) :=
+  {| arbitrarySizeST :=
+       fix gen_mem n :=
+         match n with
+         | 0 => returnGen (Some ([], empty, [], [], empty_state))
+         | S n' => (* local (lid_of_Z n) *)
+           do! m_opt <- gen_mem n';
+           match m_opt with
+           | Some (idents, c, e, m, s) => 
+             do! ident <- arbitrary;
+             do! label_id <- arbitrary;
+             do! contents <- arbitrary;
+             let addr := n in (* deterministic, always appending *)
+             let label_id := if Z.leb bound label_id then bound else label_id in
+             let idents' := ident :: idents in
+             let c' := update c ident (local (lid_of_Z label_id)) in
+             let e' := add_env_Z label_id (DVALUE_Addr addr) e in
+             let m' := m ++ [DVALUE_I64 contents] in
+             let s' := t_update s ident contents in
+             returnGen (Some (idents', c', e', m', s'))
+           | None => returnGen None
+           end
+         end
+  |}.
+
+Definition check_compile_aexp_correct_simple2A :=
+  forAll arbitrary
+         (fun (a : aexp) => 
+         forAll (genST (fun bundle => satisfies_memory_invariant_and_bound bundle 0)%Z)
+         (fun bundle =>
+            match bundle with
+            | None => checker true
+            | Some (vars, g, e, mem, st) =>
+              let result := compile_aexp g a (0, 0, [])%Z in
+              match result with
+              | ((n', m', cd'), inr v) =>
+                let cd_a := get_compiled_prefix [] cd' in
+                match cd_a with
+                | None => whenFail "not monotonic" false
+                | Some cd_a =>
+                  let c_a := compiled_code_of cd_a in
+                  match c_a with
+                  | None => whenFail "compiled result not well-formed" false
+                  | Some c_a =>
+                    match build_mcfg cd_a with
+                    | None => checker true
+                    | Some mcfg =>
+                      forAll arbitrary
+                             (fun (k : stack) => forAll arbitrary
+                             (fun (fn : function_id) => forAll arbitrary
+                             (fun (bid : block_id) => forAll arbitrary
+                             (fun phis => forAll arbitrary
+                             (fun term =>
+                                step_code_bool
+                                  mcfg
+                                  (aexp_correct_relation_bool2 vars g e st n' v
+                                                               (aeval st a)
+                                                               k fn bid phis term)
+                                  (List.rev c_a)
+                                  (slc_pc fn bid phis term c_a, e, k)
+                                  mem)))))
+                    end
+                  end
+                end
+              | _ => whenFail "couldn't compile" true
+              end
+            end)).
+
+(*! QuickChick check_compile_aexp_correct_simple2A. *)
+
+Instance show_mcfg : Show mcfg := {| show x := "(show mcfg not implemented)" |}.
+
+(*
+Definition is_env_extends (e e' : env) : Decidable (env_extends e e').
+Proof.
+  induction e; unfold Decidable.
+  - left. unfold env_extends.
+    intros op t dv eval_op_empty.
+    destruct op; destruct e; inversion eval_op_empty.
+    destruct t; simpl in *.
+   ;
+    
+  match e with
+  | [] => inl _
+  | [] => 
+*)
+
+Derive ArbitrarySizedSuchThat for (fun (instr : instr) => is_Op instr).
+Derive ArbitrarySizedSuchThat for (fun (instr : instr) => is_Eff instr).
+
+(* 
+QuickChickDebug Debug On. 
+Print GenSizedSuchThatis_Op.
+Print Hint GenSizedSuchThat. 
+Sample (@arbitraryST instr (fun instr => is_Op instr) _).
+*)
+
+(* Derive ArbitrarySizedSuchThat for (fun code => straight code)). *)
+
+Instance gen_straight_code : GenSizedSuchThat code (fun c => straight c) :=
+  {| arbitrarySizeST :=
+       fix gen_straight_code n :=
+         match n with
+         | 0 => returnGen (Some [])
+         | S n' =>
+           doM! tl <- gen_straight_code n';
+           do! id <- arbitrary;
+           doM! instr <- genST (fun i => is_Op i);
+           returnGen (Some ((id, instr) :: tl))
+         end
+  |}.
+
+Fixpoint is_Op_bool (i : instr) : bool :=
+  match i with
+  | INSTR_Op _ => true
+  | _ => false
+  end.
+
+Fixpoint is_Eff_bool (i : instr) : bool :=
+  match i with
+  | INSTR_Alloca _ _ _ => true
+  | INSTR_Load _ _ _ _ => true
+  | INSTR_Store _ _ _ _ => true
+  | _ => false
+  end.
+
+Fixpoint straight_bool (c : code) : bool :=
+  match c with
+  | [] => true
+  | ((id, i) :: c') =>
+    if orb (is_Op_bool i) (is_Eff_bool i) then straight_bool c'
+    else false
+  end.
+
+Fixpoint compiled_code_bool elts code : bool :=
+  match elts, code with
+  | [], [] => true
+  | (I id instr :: tl), ((id', instr') :: cd)  =>
+    if id == id' then
+      if instr == instr' then
+        compiled_code_bool tl cd
+      else false
+    else false
+  | _, _ => false
+  end.
 
 (* Derive ArbitrarySizedSuchThat for (fun env => env_lt n env). *)
 
+Instance gen_env_lt (bound : int) :
+  GenSizedSuchThat env (fun env => env_lt bound env) :=
+  
+  {| arbitrarySizeST :=
+       fix gen_env_lt n :=
+         match n with
+         | 0 => returnGen (Some [])
+         | S n' =>
+           do! n <- arbitrary;
+           do! dv <- arbitrary;
+           let m := if Z.leb bound n then bound else n in
+           do! env_opt <- gen_env_lt n';
+           match env_opt with
+           | Some env' =>
+             returnGen (Some (add_env_Z m dv env'))
+           | None =>
+             returnGen None
+           end
+         end
+  |}.
+
+
+(* 
+Sample (genST (fun m => satisfies_memory_invariant_and_bound m 3)%Z).
+Sample (@arbitrary stack _) 
+Sample (@arbitrary function_id _).
+Sample (@arbitrary block_id _).
+Sample (@arbitrary instr_id _).
+Sample (@arbitrary phi _).
+Sample (@arbitrary terminator _).
+Sample (@arbitrary code _).
+ *)
+
 (*
-Import Vellvm.ImpCorrectness.
-Require Import Vellvm.MemoryQuickChick.
-Sample (@arbitrarySizeST _ (fun x => is_Op x) GenSizedSuchThatis_Op 3).
+Definition check_compile_aexp_correct :=
+  forAll arbitrary
+         (fun (a : aexp) => forAll arbitrary
+         (fun (st : Imp.state) =>
+         forAll (genST (fun bundle => satisfies_memory_invariant_and_bound bundle 3)%Z)
+         (fun bundle =>
+            match bundle with
+            | None => checker true
+            | Some (vars, g, env, mem, state) =>
+              let result := compile_aexp g a (0, 0, [])%Z in
+              match result with
+              | ((n', m', cd'), inr v) =>
+                forAll arbitrary
+                       (fun (k : stack) => forAll arbitrary
+                       (* (fun (CFG : mcfg) => forAll arbitrary *)
+                       (fun (fn : function_id) => forAll arbitrary
+                       (fun (bid : block_id) => forAll arbitrary
+                       (fun phis => forAll arbitrary
+                       (fun term =>
+                          step_code_checker
+                            CFG
+                            (fun s' mem' =>
+                               let '(pc', e', k') := s' in
+                               (* pc' == slc_pc fn bid phis term [] *)
+                               check_memory_invariant_and_bound (, g, e', mem', ) n'
+                       )))))
+              | _ => checker false
+              end
+                        end))).
+*)
+          
 
-Sample (genST (fun i => is_Op i)).
+(*
+Inductive fooP : nat -> Foo -> Prop.
+Instance dec_dooP n : Dec (foo n).
 
-Derive ArbitrarySizedSuchThat for (fun instr => is_Eff instr).
-Derive ArbitrarySizedSuchThat for (fun instr => is_Op instr).
-Derive ArbitrarySizedSuchThat for (fun instr => is_Op instr).
-Derive ArbitrarySizedSuchThat for (fun instr => is_Op instr).
+if (fooP 42)? then ...
+else ...
 
+pp
+*)
 
-
-
-(* Print env_lt. *)
-
+(*
 From QuickChick Require Import QuickChick.
 Local Open Scope nat.
 Import Ollvm_ast.
 Derive Arbitrary for Expr
 Derive Arbitrary for value.
-
-Derive ArbitrarySizedSuchThat for (fun i => is_Op i).
-
-Derive ArbitrarySizedSuchThat for (fun instr => is_Op instr).
 
 *)
 
@@ -130,11 +722,3 @@ Derive ArbitrarySizedSuchThat for (fun instr => is_Op instr).
 (* Sample (genST (fun env => env_tl env)). *)
 
 (* Derive ArbitrarySizedSuchThat for (fun instr => is_Op instr). *)
-
-(*
-Lemma env_extends_lt :
-  forall e n dv
-    (Henv: env_lt n e),
-    env_extends e (add_env_Z n dv e).
-*)
-
